theories/models/utp_vdm_new/utp_vdm.thy
@@ -1,0 +1,82 @@
+(******************************************************************************)
+(* Project: VDM model for Isabelle/UTP                                        *)
+(* File: utp_vdm.thy                                                          *)
+(* Authors: Original CML model by Simon Foster, University of York (UK)       *)
+(*          Adapted to VDM by Luis Diogo Couto, Aarhus University (DK)        *)
+(******************************************************************************)
+
+theory utp_vdm
+imports
+  utp_vdm_model
+  utp_vdm_inject
+  utp_vdm_sorts
+  utp_vdm_expr
+  utp_vdm_laws
+  utp_vdm_monad
+  utp_vdm_tac
+  utp_vdm_types
+  utp_vdm_functions
+  utp_vdm_records
+  utp_vdm_stmt
+  utp_vdm_commands
+begin 
+
+text {* Remove syntax which will likely clash *}
+
+hide_const "SUB" "floor" "greatest" "Set.empty" "Map.empty" "Id" 
+           "size" "top" "top_class.top" "bot_class.bot"
+
+no_notation
+  J_pred ("J") and
+  relcomp (infixr "O" 75)
+
+(* Remove standard HOL arithmetic operators *)
+
+no_notation
+  plus (infixl "+" 65) and
+  minus (infixl "-" 65) and
+  times (infixl "*" 70) and
+  uminus ("- _" [81] 80) and
+  divide (infixl "'/" 70) and
+  Groups.zero ("0") and
+  greater_eq  (infix ">=" 50) and
+  greater  (infix ">" 50) and
+  less_eq  ("op <=") and
+  less_eq  ("(_/ <= _)" [51, 51] 50) and
+  less  ("op <") and
+  less  ("(_/ < _)"  [51, 51] 50) and
+  TrueP ("true") and
+  FalseP ("false") and
+  VarA ("&_") and
+  TrueAE ("true") and
+  FalseAE ("false") and
+  Sublist.parallel (infixl "\<parallel>" 50) and
+  utp_designs_sig.ParallelD (infixr "\<parallel>" 100)
+
+no_syntax
+  "_n_upred_assigns"    :: "n_pvars \<Rightarrow> n_pexprs \<Rightarrow> n_upred" ("_ := _" [100] 100)
+  "_n_upred_ifthenelse" :: "n_upred \<Rightarrow> n_upred \<Rightarrow> n_upred \<Rightarrow> n_upred" ("if _ then _ else _")
+  "_n_upred_while"      :: "n_upred \<Rightarrow> n_upred \<Rightarrow> n_upred" ("while _ do _ od")
+  "_upred_prefixed"     :: "n_pexpr \<Rightarrow> n_upred \<Rightarrow> n_upred" ("_ -> _")
+  "_n_upred_index"      :: "('b \<Rightarrow> 'a upred) \<Rightarrow> 'b \<Rightarrow> n_upred" ("_<_>" 50)
+  "_n_upred_var"        :: "idt \<Rightarrow> n_upred" ("_")
+  "_upred_StopCSP"      :: "n_upred" ("STOP")
+  "_upred_SkipCSP"      :: "n_upred" ("SKIP")
+  "_upred_ChaosCSP"     :: "n_upred" ("CHAOS")
+  "_n_upred_PrefixSkipCSP" :: "n_pexpr \<Rightarrow> n_upred" ("@_")
+  "_upred_callpr"          :: "('a, 'b, 'm) WF_POPERATION \<Rightarrow> n_pexpr \<Rightarrow> n_upred" ("call _'[_']")
+  "_upred_assignpr"        :: "('a, 'm) pvar \<Rightarrow> ('a, 'b, 'm) WF_POPERATION \<Rightarrow> n_pexpr \<Rightarrow> n_upred" ("_ := _'[_']" [100] 100)
+
+declare EvalD_vexpr_set_range [evalp del]
+
+(*
+vdmacts
+  P = "i:@int @ P<&i>" and
+  Q = "i:@int @ P<5 + &i>" and
+  R = "Q<1>" and
+  S = "let x : @nat = 5 in SKIP"
+
+term "ActionBlock"
+*)
+
+end
