theories/models/utp_vdm_new/utp_vdm_laws.thy
@@ -1,0 +1,147 @@
+(******************************************************************************)
+(* Project: VDM model for Isabelle/UTP                                        *)
+(* File: utp_vdm_laws.thy                                                     *)
+(* Authors: Original CML model by Simon Foster, University of York (UK)       *)
+(*          Adapted to VDM by Luis Diogo Couto, Aarhus University (DK)        *)
+(******************************************************************************)
+
+header {* Extra laws for VDM *}
+
+theory utp_vdm_laws
+imports
+  utp_vdm_expr
+  utp_vdm_functions
+begin
+
+lemma Nats_elim [elim!]:
+  "\<lbrakk> (x::real) \<in> Nats; \<lbrakk> x \<in> Ints; x \<ge> 0 \<rbrakk> \<Longrightarrow> P \<rbrakk> \<Longrightarrow> P"
+  by (auto simp add:Nats_def)
+
+lemma Nats_floor [intro]: 
+  "\<lbrakk> x \<ge> 0 \<rbrakk> \<Longrightarrow> real (hol_floor (x :: real)) \<in> Nats"
+  apply (auto simp add: Nats_def)
+  apply (metis of_nat_nat rangeI real_eq_of_int zero_le_floor)
+done
+
+lemma Nats_Ints_intro [intro!]: 
+  "\<lbrakk> (x::real) \<in> Ints; x \<ge> 0 \<rbrakk> \<Longrightarrow> x \<in> Nats"
+  apply (auto simp add:Ints_def Nats_def)
+  apply (metis Nats_def of_nat_in_Nats of_nat_nat)
+done
+
+lemma Nats_abstract [simp]: 
+  "0 \<le> real (n::nat) \<longleftrightarrow> 0 \<le> n"
+  "1 \<le> real (n::nat) \<longleftrightarrow> 1 \<le> n"
+  "(numeral m) \<le> real (n::nat) \<longleftrightarrow> numeral m \<le> n"
+  "real (n :: nat) \<le> 0 \<longleftrightarrow> n \<le> 0"
+  "real (n :: nat) \<le> 1 \<longleftrightarrow> n \<le> 1"
+  "real (n::nat) \<le> (numeral m) \<longleftrightarrow>  n \<le> numeral m"
+  apply (auto)
+  apply (metis real_of_nat_le_iff real_of_nat_numeral)
+  apply (metis natceiling_le_eq natceiling_numeral_eq)
+  apply (metis real_of_nat_le_iff real_of_nat_numeral)
+  apply (metis real_of_nat_le_iff real_of_nat_numeral)
+done
+
+lemma Ints_floor [intro]: 
+  "hol_floor (x :: real) \<in> Ints"
+  by (metis Ints_diff Ints_of_nat int_diff_cases)
+
+(* This law allows integers in VDM (elements of Ints) to
+   be converted to HOL typed integers. This has the 
+   advantage that HOL laws can be applied. *)
+
+lemma Ints_elim [elim!]:
+  "\<lbrakk> x \<in> \<int>; \<And> (y :: int). \<lbrakk> x = real y \<rbrakk> \<Longrightarrow> P \<rbrakk> \<Longrightarrow> P"
+  by (metis Ints_cases real_eq_of_int)
+
+(* The following laws are present in the default simplier
+   but in reverse. However for VDM we will often need to
+   convert a real to an integer/nat so we can take advantage
+   of HOL laws. Need to decide the best strategy for
+   dealing with this. Do we always want to convert VDM
+   types to HOL types through these abstractions? Need to
+   experiment... *)
+
+lemma Ints_abstract:
+  "(0::real) = real (0 :: int)"
+  "(numeral n) = real ((numeral n) :: int)"
+  "(plus (real (x :: int)) (real y)) = real (plus x y)"
+  "(minus (real (x :: int)) (real y)) = real (minus x y)"
+  "real (x::int) \<le> real y \<longleftrightarrow> x \<le> y"
+  "real (x::int) = real y \<longleftrightarrow> x = y"
+  "real (x::int) \<in> Nats \<longleftrightarrow> x \<ge> 0"
+  by (auto)
+
+lemma Ex_Nats [simp]: "(\<exists> x. x \<in> Nats \<and> P(x)) \<longleftrightarrow> (\<exists> n::nat. P(real n))"
+  by (metis Nats_cases Nats_real_of_nat real_of_nat_def)
+
+lemma Ex_Ints [simp]: "(\<exists> x. x \<in> Ints \<and> P(x)) \<longleftrightarrow> (\<exists> n::int. P(real n))"
+  by (metis Ints_elim Ints_real_of_int)
+
+
+lemma vallI [intro!]: "\<lbrakk> \<And> x. x \<in> A \<Longrightarrow> TautDE (F(x)) \<rbrakk> \<Longrightarrow> ForallD A F"
+  by (utp_poly_tac)
+
+lemma vexI [intro]: "\<lbrakk> x \<in> A; TautDE (F(x)) \<rbrakk> \<Longrightarrow> ExistsD A F"
+  by (utp_poly_auto_tac)
+
+lemma vinvI [intro!]: "\<lbrakk> x \<in> A; TautDE (F(x)) \<rbrakk> \<Longrightarrow> x \<in> InvS A F"
+  by (utp_poly_tac)
+
+lemma ApplyD_fun_taut [intro!]: "TautDE (f(v)) \<Longrightarrow> TautDE (ApplyD_fun f (LitD v))"
+  by (simp add:TautDE_def evalp)
+
+lemma HasType_bool_taut [simp]: "|@P : @bool| = |@P|"
+  by (auto simp add:evalp)
+
+  (*
+lemma vin_set_rangeI [intro!]:
+  "\<lbrakk> x \<in> Ints; |&x >= &m|; |&x <= &n| \<rbrakk> \<Longrightarrow> |&x in @set {&m,...,&n}|"
+  apply (auto elim!:Ints_elim simp add:evalp batLeastAtMost.rep_eq)
+  apply (rule imageI)
+  apply (auto)
+  apply (metis eq_iff floor_real_of_int linear real_le_floor)
+  apply (metis le_floor)
+done
+*)
+
+lemma vleqI [intro]: "x \<le> y \<Longrightarrow> |&x <= &y|"
+  by (utp_poly_tac)
+
+  (*
+lemma vinset_range [simp]:
+  "|&i in @set {&m,...,&n}| = |&i hasType @int and &i >= floor(&m) and &i <= floor(&n)|"
+  by (auto simp add:evalp batLeastAtMost.rep_eq)
+*)
+
+(*
+lemma vinset_rangeI [intro]:
+  "\<lbrakk> |&i hasType @int|; |&i >= floor(&m)|; |&i <= floor(&n)| \<rbrakk> \<Longrightarrow> |&i in @set {&m,...,&n}|"
+  by (auto simp add:evalp batLeastAtMost.rep_eq)
+*)
+  
+lemma hasType_inter [simp]:
+  "|@x hasType A and (@x hasType B and @P)| = |@x hasType (A \<inter> B) and @P|"
+  apply (utp_poly_tac) 
+  apply (metis (full_types) mconj_simps(1) mconj_simps(2))
+done
+
+(*
+lemma hasType_range [simp]:
+  "|&x hasType @int and &x in @set {&m,...,&n}| = |&x in @set {&m,...,&n}|"
+  by (utp_poly_tac)
+*)
+  
+(*
+lemma "|exists x : @A @ &x in @set {&m,...,&n}| \<longleftrightarrow> m \<le> n"
+  sledgehammer
+  apply (simp add:evalp)
+*)
+
+(* This causes problems so I've disabled it from the tactic for now *)
+
+declare EvalD_vexpr_set_range [evalp del]
+
+end
+
