theories/models/utp_vdm_new/utp_vdm_tac.thy
@@ -1,0 +1,132 @@
+(******************************************************************************)
+(* Project: VDM model for Isabelle/UTP                                        *)
+(* File: utp_vdm_tac.thy                                                      *)
+(* Author: Simon Foster, University of York (UK)                              *)
+(* Authors: Original CML model by Simon Foster, University of York (UK)       *)
+(*          Adapted to VDM by Luis Diogo Couto, Aarhus University (DK)        *)
+(******************************************************************************)
+
+header {* Proof Tactic for VDM *}
+
+theory utp_vdm_tac
+imports 
+  utp_vdm_expr
+begin
+
+text {* Theorem Attributes *}
+
+ML {*
+  structure vdmty_defs =
+    Named_Thms (val name = @{binding vdmty_defs} val description = "VDM type defs")
+*}
+
+ML {*
+  structure vdmval_defs =
+    Named_Thms (val name = @{binding vdmval_defs} val description = "VDM value defs")
+*}
+
+ML {*
+  structure vdmfun_defs =
+    Named_Thms (val name = @{binding vdmfun_defs} val description = "VDM function defs")
+*}
+
+ML {*
+  structure vdmop_defs =
+    Named_Thms (val name = @{binding vdmop_defs} val description = "VDM operation defs")
+*}
+
+setup vdmty_defs.setup
+setup vdmval_defs.setup
+setup vdmfun_defs.setup
+setup vdmop_defs.setup
+
+
+ML {*
+  fun utp_vdm_defs ctxt =
+    ctxt
+      addsimps (vdmty_defs.get ctxt)
+      addsimps (vdmval_defs.get ctxt)
+      addsimps (vdmfun_defs.get ctxt)
+      addsimps (vdmop_defs.get ctxt)
+*}
+
+ML {*
+  fun utp_vdm_simpset ctxt =
+    (utp_vdm_defs ctxt)
+      addsimps (evalp.get ctxt)
+      addsimps (evalpp.get ctxt)
+      addsimps (closure.get ctxt)
+      addsimps (typing.get ctxt)
+      addsimps (defined.get ctxt);
+*}
+
+ML {*
+  fun utp_vdm_unfold_tac thms ctxt i =
+    CHANGED (
+      TRY (asm_full_simp_tac (utp_vdm_defs ctxt) i))
+*}
+
+ML {*
+  fun utp_vdm_tac thms ctxt i =
+    CHANGED (
+      TRY (asm_full_simp_tac (utp_vdm_simpset ctxt) i))
+*}
+
+ML {*
+  fun utp_vdm_auto_tac thms ctxt i =
+    CHANGED ((
+      (asm_full_simp_tac (utp_vdm_simpset ctxt)) THEN_ALL_NEW
+      (asm_full_simp_tac ctxt) THEN_ALL_NEW
+      (SELECT_GOAL (auto_tac ctxt))) i)
+*}
+
+method_setup unfold_vdm = {*
+  Attrib.thms >>
+  (fn thms => fn ctxt =>
+    SIMPLE_METHOD' (utp_vdm_unfold_tac thms ctxt))
+*} "proof tactic for VDM"
+
+method_setup vdm_tac = {*
+  Attrib.thms >>
+  (fn thms => fn ctxt =>
+    SIMPLE_METHOD' (utp_vdm_tac thms ctxt))
+*} "proof tactic for VDM"
+
+method_setup vdm_auto_tac = {*
+  Attrib.thms >>
+  (fn thms => fn ctxt =>
+    SIMPLE_METHOD' (utp_vdm_auto_tac thms ctxt))
+*} "proof tactic for predicates with auto"
+
+text {* Set up some simplifications to deal with finite sets and strings *}
+
+declare nibble_less_eq_def [simp]
+declare nibble_less_def [simp]
+
+text {* Some examples *}
+
+lemma mimplies_Some_Some [simp]:
+  "mimplies (Some x) (Some y) = Some (x \<longrightarrow> y)"
+  by (case_tac x, auto)
+
+(*
+lemma vdm_goal1:
+  "|forall x : @bool @ &x => &x| = |true|"
+  by (vdm_auto_tac)
+
+lemma vdm_goal2:
+  "|forall x : @nat1 @ &x > 0| = |true|"
+  by (vdm_tac)
+
+lemma vdm_goal3:
+  "|forall x : @nat @ (&x < 5) => &x in @set {0,1,2,3,4}| = |true|"
+  oops
+
+lemma vdm_goal4: "|iota x : @nat @ &x = 5| = |5|"
+  by (vdm_auto_tac)
+*)
+
+declare fcard_def [evalp]
+declare blist.rep_eq [evalp]
+
+end
